Printf for Low*

ulib/LowStar.Printf.fst
@@ -15,16 +15,103 @@
 *)
 module LowStar.Printf
 
+/// This module provides imperative printing functions for several
+/// primitive Low* types, including
+///  -- booleans (%b)
+///  -- characters (%c)
+///  -- strings (%s)
+///  -- machine integers
+///          (UInt8.t as %uy, UInt16.t as %us, UInt32.t as %ul, and UInt64.t as %uL;
+///            Int8.t  as %y,  Int16.t as %i,   Int32.t as %l , and  Int64.t as %L)
+///  -- and arrays (aka buffers) of these base types formatted
+///         as %xN, where N is the format specifier for the array element type
+///         e.g., %xuy for buffers of UInt8.t
+
+/// The main function of this module is `printf`
+/// There are a few main differences relative to C printf
+///   -- The format specifiers are different (see above)
+///
+///   -- For technical reasons explained below, an extra dummy
+///      argument `done` has to be provided at the end for the
+///      computation to have any effect.
+///
+///      E.g., one must write
+///           `printf "%b %c" true 'c' done`
+///      rather than just
+///           `printf "%b %c" true 'c'`
+///
+///   -- When printing arrays, two arguments must be passed; the
+///      length of the array fragment to be formatted and the array
+///      itself
+///
+///   -- When extracted, rather than producing a C `printf` (which
+///      does not, e.g., support printing of dynamically sized
+///      arrays), our `printf` is specialized to a sequence of calls
+///      to primitive printers for each supported type
+///
+/// Before diving into the technical details of how this module works,
+/// you might want to skip to the very end of this file to see a
+/// small piece of sample code and how it extracts.
+
 open FStar.Char
 open FStar.String
+open FStar.HyperStack.ST
 module L = FStar.List.Tot
 module LB = LowStar.Monotonic.Buffer
-module I = FStar.Integers
 
-irreducible
+/// `lmbuffer a r s l` is
+///    - a monotonic buffer of `a`
+///    - governed by preorders `r` and `s`
+///    - with length `l`
+let lmbuffer a r s l =
+    b:LB.mbuffer a r s{
+      LB.len b == l
+    }
+
+/// `StTrivial`: A effect abbreviation for a stateful computation
+///  with no precondition, and which does not change the state
+effect StTrivial (a:Type) =
+  Stack a
+    (requires fun h -> True)
+    (ensures fun h0 _ h1 -> h0==h1)
+
+/// `StBuf a b`: A effect abbreviation for a stateful computation
+///  that may read `b` does not change the state
+effect StBuf (a:Type) #t #r #s #l (b:lmbuffer t r s l) =
+  Stack a
+    (requires fun h -> LB.live h b)
+    (ensures (fun h0 _ h1 -> h0 == h1))
+
+/// Primitive printers for all the types supported by this module
+assume val print_string: string -> StTrivial unit
+assume val print_char  : char -> StTrivial unit
+assume val print_u8  : UInt8.t -> StTrivial unit
+assume val print_u16 : UInt16.t -> StTrivial unit
+assume val print_u32 : UInt32.t -> StTrivial unit
+assume val print_u64 : UInt64.t -> StTrivial unit
+assume val print_i8  : Int8.t -> StTrivial unit
+assume val print_i16 : Int16.t -> StTrivial unit
+assume val print_i32 : Int32.t -> StTrivial unit
+assume val print_i64 : Int64.t -> StTrivial unit
+assume val print_bool : bool -> StTrivial unit
+assume val print_lmbuffer_bool (l:_) (#r:_) (#s:_) (b:lmbuffer bool r s l) : StBuf unit b
+assume val print_lmbuffer_char (l:_) (#r:_) (#s:_) (b:lmbuffer char r s l) : StBuf unit b
+assume val print_lmbuffer_u8 (l:_) (#r:_) (#s:_) (b:lmbuffer UInt8.t r s l) : StBuf unit b
+assume val print_lmbuffer_u16 (l:_) (#r:_) (#s:_) (b:lmbuffer UInt16.t r s l) : StBuf unit b
+assume val print_lmbuffer_u32 (l:_) (#r:_) (#s:_) (b:lmbuffer UInt32.t r s l) : StBuf unit b
+assume val print_lmbuffer_u64 (l:_) (#r:_) (#s:_) (b:lmbuffer UInt64.t r s l) : StBuf unit b
+assume val print_lmbuffer_i8 (l:_) (#r:_) (#s:_) (b:lmbuffer Int8.t r s l) : StBuf unit b
+assume val print_lmbuffer_i16 (l:_) (#r:_) (#s:_) (b:lmbuffer Int16.t r s l) : StBuf unit b
+assume val print_lmbuffer_i32 (l:_) (#r:_) (#s:_) (b:lmbuffer Int32.t r s l) : StBuf unit b
+assume val print_lmbuffer_i64 (l:_) (#r:_) (#s:_) (b:lmbuffer Int64.t r s l) : StBuf unit b
+
+
+/// An attribute to control reduction
+noextract irreducible
 let __reduce__ = unit
 
-noeq
+/// Base types supported so far
+noextract
 type base_typ =
   | Bool
   | Char
@@ -37,12 +124,15 @@ type base_typ =
   | I32
   | I64
 
-noeq
+/// Argument types are base types and arrays thereof
+noextract
 type arg =
   | Base of base_typ
   | Array of base_typ
 
+/// Interpreting a `base_typ` as a type
 [@__reduce__]
+noextract
 let base_typ_as_type (b:base_typ) : Type0 =
   match b with
   | Bool   -> bool
@@ -56,19 +146,22 @@ let base_typ_as_type (b:base_typ) : Type0 =
   | I32    -> FStar.Int32.t
   | I64    -> FStar.Int64.t
 
-noeq
+/// `fragment`: A format string is parsed into a list of fragments of
+///  string literals and other arguments that need to be spliced in
+///  (interpolated)
+noextract
 type fragment =
   | Frag of string
   | Interpolate of arg
 
+noextract
 let fragments = list fragment
 
-let cons_char (c:char) (s:string) = string_of_list (c :: list_of_string s)
-
 /// `parse_format s`:
-///     Parses a list of characters into a list of directives
+///     Parses a list of characters in a format string into a list of fragments
 ///     Or None, in case the format string is invalid
 [@__reduce__]
+noextract inline_for_extraction
 let rec parse_format
       (s:list char)
  : Tot (option fragments)
@@ -85,7 +178,7 @@ let rec parse_format
    in
    let cons_frag (c:char) (ods:option fragments)
      = match ods with
-       | Some (Frag s::rest) -> Some (Frag (cons_char c s) :: rest)
+       | Some (Frag s::rest) -> Some (Frag (string_of_list (c :: list_of_string s)) :: rest)
        | Some rest -> Some (Frag (string_of_list [c]) :: rest)
        | _ -> None
    in
@@ -94,7 +187,7 @@ let rec parse_format
    | ['%'] -> None
 
    // %x... arrays of base types
-   | '%' :: 'x' :: s' -> 
+   | '%' :: 'x' :: s' ->
      head_buffer (parse_format ('%' :: s'))
 
    // %u ... Unsigned integers
@@ -124,47 +217,91 @@ let rec parse_format
      cons_frag c (parse_format s')
 
 
-/// `parse_format_string`: parses a format `string` into a list of directives
+/// `parse_format_string`: a wrapper around `parse_format`
 [@__reduce__]
+noextract inline_for_extraction
 let parse_format_string
     (s:string)
   : option fragments
   = parse_format (list_of_string s)
 
-open FStar.HyperStack.ST
-abstract
+/// `lift a` lifts the type `a` to a higher universe
+noextract
 type lift (a:Type u#a) : Type u#(max a b) =
   | Lift : a -> lift a
-  
+
+/// `done` is a `unit` in universe 1
+noextract
 let done : lift unit = Lift u#0 u#1 ()
 
+/// `arg_t`: interpreting an argument as a type
+///   (in universe 1) since it is polymorphic in the preorders of a buffer
 [@__reduce__]
-let rec interpret_args (l:fragments) (acc:list LB.buf_t) : Type u#1 =
+noextract
+let rec arg_t (a:arg) : Type u#1 =
+  match a with
+  | Base t -> lift (base_typ_as_type t)
+  | Array t -> (l:UInt32.t & r:_ & s:_ & lmbuffer (base_typ_as_type t) r s l)
+
+
+/// `frag_t`: a fragment is either a string literal or a argument to be interpolated
+noextract
+let frag_t = either string (a:arg & arg_t a)
+
+/// `live_frags h l` is a liveness predicate on all the buffers in `l`
+[@__reduce__]
+noextract
+let rec live_frags (h:_) (l:list frag_t) : prop =
+  match l with
+  | [] -> True
+  | Inl _ :: rest -> live_frags h rest
+  | Inr a :: rest ->
+    (match a with
+     | (| Base _, _ |) -> live_frags h rest
+     | (| Array _, (| _, _, _, b |) |) -> LB.live h b /\ live_frags h rest)
+
+
+/// `interpret_frags` interprets a list of fragments as a Low* function type
+///    Note `l` is the fragments in L-to-R order (i.e., parsing order)
+///    `acc` accumulates the fragment values in reverse order
+[@__reduce__]
+noextract
+let rec interpret_frags (l:fragments) (acc:list frag_t) : Type u#1 =
   match l with
   | [] ->
+    // Always a dummy argument at the end
+    // Ensures that all cases of this match
+    // have the same universe, i.e., u#1
      lift u#0 u#1 unit
     -> Stack unit
-      (requires (fun h0 -> 
-          FStar.BigOps.big_and' #LB.buf_t (fun (| _, _, _, b |) -> LB.live h0 b) acc))
-      (ensures (fun h0 _ h1 -> h0 == h1))
+      (requires fun h0 -> live_frags h0 acc)
+      (ensures fun h0 _ h1 -> h0 == h1)
 
   | Interpolate (Base t) :: args ->
-    base_typ_as_type t ->
-    interpret_args args acc
+    // Base types are simple: we just take one more argument
+    x:base_typ_as_type t ->
+    interpret_frags args (Inr (| Base t, Lift x |) :: acc)
 
   | Interpolate (Array t) :: args ->
-    l:UInt32.t -> 
-    #r:_ ->
-    #s:_ ->
-    b:LB.mbuffer (base_typ_as_type t) r s ->
-    interpret_args args (LB.buf b :: acc)
+    // Arrays are implicitly polymorphic in their preorders `r` and `s`
+    // which is what forces us to be in universe 1
+    // Note, the length `l` is explicit
+    l:UInt32.t ->
+    #r:LB.srel (base_typ_as_type t) ->
+    #s:LB.srel (base_typ_as_type t) ->
+    b:lmbuffer (base_typ_as_type t) r s l ->
+    interpret_frags args (Inr (| Array t, (| l, r, s, b |) |)  :: acc)
 
-  | Frag _ :: args ->
-    interpret_args args acc
-    
-unfold
+  | Frag s :: args ->
+    // Literal fragments do not incur an additional argument
+    // We just accumulate them and recur
+    interpret_frags args (Inl s :: acc)
+
+
+/// `normal` A normalization marker with very specific steps enabled
+noextract unfold
 let normal (#a:Type) (x:a) : a =
-  FStar.Pervasives.norm 
+  FStar.Pervasives.norm
     [iota;
      zeta;
      delta_attr [`%__reduce__; `%BigOps.__reduce__];
@@ -173,20 +310,143 @@ let normal (#a:Type) (x:a) : a =
      simplify]
      x
 
-let elim_normal (x:bool) : Lemma (requires (normal #bool x)) (ensures x) = ()
+/// `coerce`: A utility to trigger extensional equality of types
+noextract
+let coerce (x:'a{'a == 'b}) : 'b = x
 
-let rec aux (frags:fragments) : interpret_args frags
-val printf (s:string{normal #bool (Some? (parse_format_string s))})
-  : normal (interpret_args (Some?.v (parse_format_string s)) [])
-let printf s =
-  let args = parse_format_string s in
-  let rec aux a
+/// `print_frags`: Having accumulated all the pieces of a format
+/// string and the arguments to the printed (i.e., the `list frag_t`),
+/// this function does the actual work of printing them all using the
+/// primitive printers
+noextract inline_for_extraction
+let rec print_frags (acc:list frag_t)
+  : Stack unit
+        (requires fun h0 -> live_frags h0 acc)
+        (ensures fun h0 _ h1 -> h0 == h1)
+  = match acc with
+    | [] -> ()
+    | hd::tl ->
+      print_frags tl;
+      (match hd with
+       | Inl s -> print_string s
+       | Inr (| Base t, Lift value |) ->
+         (match t with
+           | Bool -> print_bool value
+           | Char -> print_char value
+           | U8 ->   print_u8 value
+           | U16 ->  print_u16 value
+           | U32 ->  print_u32 value
+           | U64 ->  print_u64 value
+           | I8 ->   print_i8 value
+           | I16 ->  print_i16 value
+           | I32 ->  print_i32 value
+           | I64 ->  print_i64 value)
+       | Inr (| Array t, (| l, r, s, value |) |) ->
+         (match t with
+           | Bool ->  print_lmbuffer_bool l value
+           | Char -> print_lmbuffer_char l value
+           | U8 ->   print_lmbuffer_u8 l value
+           | U16 ->  print_lmbuffer_u16 l value
+           | U32 ->  print_lmbuffer_u32 l value
+           | U64 ->  print_lmbuffer_u64 l value
+           | I8 ->   print_lmbuffer_i8 l value
+           | I16 ->  print_lmbuffer_i16 l value
+           | I32 ->  print_lmbuffer_i32 l value
+           | I64 ->  print_lmbuffer_i64 l value))
 
+/// `aux frags acc`: This is the main workhorse which interprets a
+/// parsed format string (`frags`) as a variadic, stateful function
+[@__reduce__]
+noextract inline_for_extraction
+let rec aux (frags:fragments) (acc:list frag_t) : interpret_frags frags acc =
+  match frags with
+  | [] ->
+    let f (l:lift u#0 u#1 unit)
+      : Stack unit
+        (requires fun h0 -> live_frags h0 acc)
+        (ensures fun h0 _ h1 -> h0 == h1)
+      = print_frags acc
+    in
+    (f <: interpret_frags [] acc)
+
+  | Frag s :: rest ->
+    coerce (aux rest (Inl s :: acc))
+
+  | Interpolate (Base t) :: args ->
+    let f (x:base_typ_as_type t)
+      : interpret_frags args (Inr (| Base t, Lift x |) :: acc)
+      = aux args (Inr (| Base t, Lift x |) :: acc)
+    in
+    f
+
+  | Interpolate (Array t) :: rest ->
+    let f :
+       l:UInt32.t
+     -> #r:LB.srel (base_typ_as_type t)
+     -> #s:LB.srel (base_typ_as_type t)
+     -> b:lmbuffer (base_typ_as_type t) r s l
+     -> interpret_frags rest (Inr (| Array t, (| l, r, s, b |) |) :: acc)
+     = fun l #r #s b -> aux rest (Inr (| Array t, (| l, r, s, b |) |) :: acc)
+    in
+    f <: interpret_frags (Interpolate (Array t) :: rest) acc
+
+/// `format_string` : A valid format string is one that can be successfully parsed
+[@__reduce__]
+noextract
+let format_string = s:string{normal #bool (Some? (parse_format_string s))}
+
+/// `interpret_format_string` parses a string into fragments and then
+/// interprets it as a type
+[@__reduce__]
+noextract
+let interpret_format_string (s:format_string) : Type =
+  interpret_frags (Some?.v (parse_format_string s)) []
+
+/// `printf'`: Almost there ... this has a variadic type
+///  and calls the actual printers for all its arguments.
+///
+///  Note, the `normalize_term` in its body is crucial. It's what
+///  allows the term to be specialized at extraction time.
+noextract inline_for_extraction
+let printf' (s:format_string) : interpret_format_string s =
+  normalize_term
+  (match parse_format_string s with
+    | Some frags -> aux frags [])
+
+/// `intro_normal_f`: a technical gadget to introduce
+/// implicit normalization in the domain and co-domain of a function type
+noextract inline_for_extraction
+let intro_normal_f (#a:Type) (b: (a -> Type)) (f:(x:a -> b x))
+  : (x:(normal a) -> normal (b x))
+  = f
+
+/// `printf`: The main function has type
+///    `s:normal format_string -> normal (interpret_format_string s)`
+/// Note:
+///   This is the type F* infers for it and it is best to leave it that way
+///   rather then writing it down and asking F* to re-check what it inferred.
+///
+///   Annotating it results in a needless additional proof obligation to
+///   equate types after they are partially reduced, which is pointless.
+noextract inline_for_extraction
+let printf = intro_normal_f #format_string interpret_format_string printf'
+
+/// `test`: A small test function
+/// Running `fstar --codegen OCaml LowStar.Printf.fst --extract LowStar.Printf`
+/// produces the following for the body of this function
+///    ```
+///            print_string "Hello ";
+///            print_bool true;
+///            print_string " Low* ";
+///            print_u64 m;
+///            print_string " Printf ";
+///            print_lmbuffer_bool l () () x
+///   ```
 let test (m:UInt64.t) (l:UInt32.t) (#r:_) (#s:_) (x:LB.mbuffer bool r s{LB.len x = l})
   : Stack unit
     (requires (fun h0 -> LB.live h0 x))
     (ensures (fun h0 _ h1 -> h0 == h1))
-  = printf "%b%uL%xb" 
+  = printf "Hello %b Low* %uL Printf %xb"
               true  //%b boolean
               m     //%uL u64
               l x   //%xb (buffer bool)
